_CoqProject is in dependency order. MAINTAIN THIS.

spec/ett.v
@@ -48,7 +48,7 @@ with tm : Set :=  (*r types and kinds *)
  | a_DataCon (K:datacon)
  | a_Case (a:tm) (brs5:brs)
  | a_Sub (R:role) (a:tm)
- | a_Coerce (a:tm)
+ | a_Coerce : tm
  | a_SrcApp (a:tm) (b:tm)
 with brs : Set :=  (*r case branches *)
  | br_None : brs
@@ -107,12 +107,76 @@ Definition sig : Set := list (atom * sig_sort).
 
 Definition Nat : Set := nat.
 
+Definition theta : Set := list ( atom * pattern_arg ).
+
 (* EXPERIMENTAL *)
 (** auxiliary functions on the new list types *)
 (** library functions *)
 (** subrules *)
 (** arities *)
 (** opening up abstractions *)
+Fixpoint open_brs_wrt_co_rec (k:nat) (g5:co) (brs_6:brs) {struct brs_6}: brs :=
+  match brs_6 with
+  | br_None => br_None 
+  | (br_One K a brs5) => br_One K (open_tm_wrt_co_rec k g5 a) (open_brs_wrt_co_rec k g5 brs5)
+end
+with open_tm_wrt_co_rec (k:nat) (g5:co) (a5:tm) {struct a5}: tm :=
+  match a5 with
+  | a_Star => a_Star 
+  | (a_Var_b nat) => a_Var_b nat
+  | (a_Var_f x) => a_Var_f x
+  | (a_Abs rho A b) => a_Abs rho (open_tm_wrt_co_rec k g5 A) (open_tm_wrt_co_rec k g5 b)
+  | (a_UAbs rho b) => a_UAbs rho (open_tm_wrt_co_rec k g5 b)
+  | (a_App a nu b) => a_App (open_tm_wrt_co_rec k g5 a) nu (open_tm_wrt_co_rec k g5 b)
+  | (a_Pi rho A B) => a_Pi rho (open_tm_wrt_co_rec k g5 A) (open_tm_wrt_co_rec k g5 B)
+  | (a_CAbs phi b) => a_CAbs (open_constraint_wrt_co_rec k g5 phi) (open_tm_wrt_co_rec (S k) g5 b)
+  | (a_UCAbs b) => a_UCAbs (open_tm_wrt_co_rec (S k) g5 b)
+  | (a_CApp a g) => a_CApp (open_tm_wrt_co_rec k g5 a) (open_co_wrt_co_rec k g5 g)
+  | (a_CPi phi B) => a_CPi (open_constraint_wrt_co_rec k g5 phi) (open_tm_wrt_co_rec (S k) g5 B)
+  | (a_Conv a R g) => a_Conv (open_tm_wrt_co_rec k g5 a) R (open_co_wrt_co_rec k g5 g)
+  | (a_Fam F) => a_Fam F
+  | a_Bullet => a_Bullet 
+  | (a_Pattern R a F Apps5 b1 b2) => a_Pattern R (open_tm_wrt_co_rec k g5 a) F Apps5 (open_tm_wrt_co_rec k g5 b1) (open_tm_wrt_co_rec k g5 b2)
+  | (a_DataCon K) => a_DataCon K
+  | (a_Case a brs5) => a_Case (open_tm_wrt_co_rec k g5 a) (open_brs_wrt_co_rec k g5 brs5)
+  | (a_Sub R a) => a_Sub R (open_tm_wrt_co_rec k g5 a)
+  | a_Coerce => a_Coerce 
+  | (a_SrcApp a b) => a_SrcApp (open_tm_wrt_co_rec k g5 a) (open_tm_wrt_co_rec k g5 b)
+end
+with open_constraint_wrt_co_rec (k:nat) (g5:co) (phi5:constraint) : constraint :=
+  match phi5 with
+  | (Eq a b A R) => Eq (open_tm_wrt_co_rec k g5 a) (open_tm_wrt_co_rec k g5 b) (open_tm_wrt_co_rec k g5 A) R
+end
+with open_co_wrt_co_rec (k:nat) (g_5:co) (g__6:co) {struct g__6}: co :=
+  match g__6 with
+  | g_Triv => g_Triv 
+  | (g_Var_b nat) => if (k === nat) then g_5 else (g_Var_b nat)
+  | (g_Var_f c) => g_Var_f c
+  | (g_Beta a b) => g_Beta (open_tm_wrt_co_rec k g_5 a) (open_tm_wrt_co_rec k g_5 b)
+  | (g_Refl a) => g_Refl (open_tm_wrt_co_rec k g_5 a)
+  | (g_Refl2 a b g) => g_Refl2 (open_tm_wrt_co_rec k g_5 a) (open_tm_wrt_co_rec k g_5 b) (open_co_wrt_co_rec k g_5 g)
+  | (g_Sym g) => g_Sym (open_co_wrt_co_rec k g_5 g)
+  | (g_Trans g1 g2) => g_Trans (open_co_wrt_co_rec k g_5 g1) (open_co_wrt_co_rec k g_5 g2)
+  | (g_Sub g) => g_Sub (open_co_wrt_co_rec k g_5 g)
+  | (g_PiCong rho R g1 g2) => g_PiCong rho R (open_co_wrt_co_rec k g_5 g1) (open_co_wrt_co_rec k g_5 g2)
+  | (g_AbsCong rho R g1 g2) => g_AbsCong rho R (open_co_wrt_co_rec k g_5 g1) (open_co_wrt_co_rec k g_5 g2)
+  | (g_AppCong g1 rho R g2) => g_AppCong (open_co_wrt_co_rec k g_5 g1) rho R (open_co_wrt_co_rec k g_5 g2)
+  | (g_PiFst g) => g_PiFst (open_co_wrt_co_rec k g_5 g)
+  | (g_CPiFst g) => g_CPiFst (open_co_wrt_co_rec k g_5 g)
+  | (g_IsoSnd g) => g_IsoSnd (open_co_wrt_co_rec k g_5 g)
+  | (g_PiSnd g1 g2) => g_PiSnd (open_co_wrt_co_rec k g_5 g1) (open_co_wrt_co_rec k g_5 g2)
+  | (g_CPiCong g1 g3) => g_CPiCong (open_co_wrt_co_rec k g_5 g1) (open_co_wrt_co_rec (S k) g_5 g3)
+  | (g_CAbsCong g1 g3 g4) => g_CAbsCong (open_co_wrt_co_rec k g_5 g1) (open_co_wrt_co_rec (S k) g_5 g3) (open_co_wrt_co_rec k g_5 g4)
+  | (g_CAppCong g g1 g2) => g_CAppCong (open_co_wrt_co_rec k g_5 g) (open_co_wrt_co_rec k g_5 g1) (open_co_wrt_co_rec k g_5 g2)
+  | (g_CPiSnd g g1 g2) => g_CPiSnd (open_co_wrt_co_rec k g_5 g) (open_co_wrt_co_rec k g_5 g1) (open_co_wrt_co_rec k g_5 g2)
+  | (g_Cast g1 R g2) => g_Cast (open_co_wrt_co_rec k g_5 g1) R (open_co_wrt_co_rec k g_5 g2)
+  | (g_EqCong g1 A g2) => g_EqCong (open_co_wrt_co_rec k g_5 g1) (open_tm_wrt_co_rec k g_5 A) (open_co_wrt_co_rec k g_5 g2)
+  | (g_IsoConv phi1 phi2 g) => g_IsoConv (open_constraint_wrt_co_rec k g_5 phi1) (open_constraint_wrt_co_rec k g_5 phi2) (open_co_wrt_co_rec k g_5 g)
+  | (g_Eta a) => g_Eta (open_tm_wrt_co_rec k g_5 a)
+  | (g_Left g g') => g_Left (open_co_wrt_co_rec k g_5 g) (open_co_wrt_co_rec k g_5 g')
+  | (g_Right g g') => g_Right (open_co_wrt_co_rec k g_5 g) (open_co_wrt_co_rec k g_5 g')
+end.
+
 Fixpoint open_co_wrt_tm_rec (k:nat) (a5:tm) (g_5:co) {struct g_5}: co :=
   match g_5 with
   | g_Triv => g_Triv 
@@ -167,86 +231,12 @@ with open_tm_wrt_tm_rec (k:nat) (a5:tm) (a_6:tm) {struct a_6}: tm :=
   | (a_DataCon K) => a_DataCon K
   | (a_Case a brs5) => a_Case (open_tm_wrt_tm_rec k a5 a) (open_brs_wrt_tm_rec k a5 brs5)
   | (a_Sub R a) => a_Sub R (open_tm_wrt_tm_rec k a5 a)
-  | (a_Coerce a) => a_Coerce (open_tm_wrt_tm_rec k a5 a)
+  | a_Coerce => a_Coerce 
   | (a_SrcApp a b) => a_SrcApp (open_tm_wrt_tm_rec k a5 a) (open_tm_wrt_tm_rec k a5 b)
 end
 with open_constraint_wrt_tm_rec (k:nat) (a5:tm) (phi5:constraint) : constraint :=
   match phi5 with
   | (Eq a b A R) => Eq (open_tm_wrt_tm_rec k a5 a) (open_tm_wrt_tm_rec k a5 b) (open_tm_wrt_tm_rec k a5 A) R
-end.
-
-Fixpoint open_co_wrt_co_rec (k:nat) (g_5:co) (g__6:co) {struct g__6}: co :=
-  match g__6 with
-  | g_Triv => g_Triv 
-  | (g_Var_b nat) => if (k === nat) then g_5 else (g_Var_b nat)
-  | (g_Var_f c) => g_Var_f c
-  | (g_Beta a b) => g_Beta (open_tm_wrt_co_rec k g_5 a) (open_tm_wrt_co_rec k g_5 b)
-  | (g_Refl a) => g_Refl (open_tm_wrt_co_rec k g_5 a)
-  | (g_Refl2 a b g) => g_Refl2 (open_tm_wrt_co_rec k g_5 a) (open_tm_wrt_co_rec k g_5 b) (open_co_wrt_co_rec k g_5 g)
-  | (g_Sym g) => g_Sym (open_co_wrt_co_rec k g_5 g)
-  | (g_Trans g1 g2) => g_Trans (open_co_wrt_co_rec k g_5 g1) (open_co_wrt_co_rec k g_5 g2)
-  | (g_Sub g) => g_Sub (open_co_wrt_co_rec k g_5 g)
-  | (g_PiCong rho R g1 g2) => g_PiCong rho R (open_co_wrt_co_rec k g_5 g1) (open_co_wrt_co_rec k g_5 g2)
-  | (g_AbsCong rho R g1 g2) => g_AbsCong rho R (open_co_wrt_co_rec k g_5 g1) (open_co_wrt_co_rec k g_5 g2)
-  | (g_AppCong g1 rho R g2) => g_AppCong (open_co_wrt_co_rec k g_5 g1) rho R (open_co_wrt_co_rec k g_5 g2)
-  | (g_PiFst g) => g_PiFst (open_co_wrt_co_rec k g_5 g)
-  | (g_CPiFst g) => g_CPiFst (open_co_wrt_co_rec k g_5 g)
-  | (g_IsoSnd g) => g_IsoSnd (open_co_wrt_co_rec k g_5 g)
-  | (g_PiSnd g1 g2) => g_PiSnd (open_co_wrt_co_rec k g_5 g1) (open_co_wrt_co_rec k g_5 g2)
-  | (g_CPiCong g1 g3) => g_CPiCong (open_co_wrt_co_rec k g_5 g1) (open_co_wrt_co_rec (S k) g_5 g3)
-  | (g_CAbsCong g1 g3 g4) => g_CAbsCong (open_co_wrt_co_rec k g_5 g1) (open_co_wrt_co_rec (S k) g_5 g3) (open_co_wrt_co_rec k g_5 g4)
-  | (g_CAppCong g g1 g2) => g_CAppCong (open_co_wrt_co_rec k g_5 g) (open_co_wrt_co_rec k g_5 g1) (open_co_wrt_co_rec k g_5 g2)
-  | (g_CPiSnd g g1 g2) => g_CPiSnd (open_co_wrt_co_rec k g_5 g) (open_co_wrt_co_rec k g_5 g1) (open_co_wrt_co_rec k g_5 g2)
-  | (g_Cast g1 R g2) => g_Cast (open_co_wrt_co_rec k g_5 g1) R (open_co_wrt_co_rec k g_5 g2)
-  | (g_EqCong g1 A g2) => g_EqCong (open_co_wrt_co_rec k g_5 g1) (open_tm_wrt_co_rec k g_5 A) (open_co_wrt_co_rec k g_5 g2)
-  | (g_IsoConv phi1 phi2 g) => g_IsoConv (open_constraint_wrt_co_rec k g_5 phi1) (open_constraint_wrt_co_rec k g_5 phi2) (open_co_wrt_co_rec k g_5 g)
-  | (g_Eta a) => g_Eta (open_tm_wrt_co_rec k g_5 a)
-  | (g_Left g g') => g_Left (open_co_wrt_co_rec k g_5 g) (open_co_wrt_co_rec k g_5 g')
-  | (g_Right g g') => g_Right (open_co_wrt_co_rec k g_5 g) (open_co_wrt_co_rec k g_5 g')
-end
-with open_brs_wrt_co_rec (k:nat) (g5:co) (brs_6:brs) {struct brs_6}: brs :=
-  match brs_6 with
-  | br_None => br_None 
-  | (br_One K a brs5) => br_One K (open_tm_wrt_co_rec k g5 a) (open_brs_wrt_co_rec k g5 brs5)
-end
-with open_tm_wrt_co_rec (k:nat) (g5:co) (a5:tm) {struct a5}: tm :=
-  match a5 with
-  | a_Star => a_Star 
-  | (a_Var_b nat) => a_Var_b nat
-  | (a_Var_f x) => a_Var_f x
-  | (a_Abs rho A b) => a_Abs rho (open_tm_wrt_co_rec k g5 A) (open_tm_wrt_co_rec k g5 b)
-  | (a_UAbs rho b) => a_UAbs rho (open_tm_wrt_co_rec k g5 b)
-  | (a_App a nu b) => a_App (open_tm_wrt_co_rec k g5 a) nu (open_tm_wrt_co_rec k g5 b)
-  | (a_Pi rho A B) => a_Pi rho (open_tm_wrt_co_rec k g5 A) (open_tm_wrt_co_rec k g5 B)
-  | (a_CAbs phi b) => a_CAbs (open_constraint_wrt_co_rec k g5 phi) (open_tm_wrt_co_rec (S k) g5 b)
-  | (a_UCAbs b) => a_UCAbs (open_tm_wrt_co_rec (S k) g5 b)
-  | (a_CApp a g) => a_CApp (open_tm_wrt_co_rec k g5 a) (open_co_wrt_co_rec k g5 g)
-  | (a_CPi phi B) => a_CPi (open_constraint_wrt_co_rec k g5 phi) (open_tm_wrt_co_rec (S k) g5 B)
-  | (a_Conv a R g) => a_Conv (open_tm_wrt_co_rec k g5 a) R (open_co_wrt_co_rec k g5 g)
-  | (a_Fam F) => a_Fam F
-  | a_Bullet => a_Bullet 
-  | (a_Pattern R a F Apps5 b1 b2) => a_Pattern R (open_tm_wrt_co_rec k g5 a) F Apps5 (open_tm_wrt_co_rec k g5 b1) (open_tm_wrt_co_rec k g5 b2)
-  | (a_DataCon K) => a_DataCon K
-  | (a_Case a brs5) => a_Case (open_tm_wrt_co_rec k g5 a) (open_brs_wrt_co_rec k g5 brs5)
-  | (a_Sub R a) => a_Sub R (open_tm_wrt_co_rec k g5 a)
-  | (a_Coerce a) => a_Coerce (open_tm_wrt_co_rec k g5 a)
-  | (a_SrcApp a b) => a_SrcApp (open_tm_wrt_co_rec k g5 a) (open_tm_wrt_co_rec k g5 b)
-end
-with open_constraint_wrt_co_rec (k:nat) (g5:co) (phi5:constraint) : constraint :=
-  match phi5 with
-  | (Eq a b A R) => Eq (open_tm_wrt_co_rec k g5 a) (open_tm_wrt_co_rec k g5 b) (open_tm_wrt_co_rec k g5 A) R
-end.
-
-Definition open_sig_sort_wrt_tm_rec (k:nat) (a5:tm) (sig_sort5:sig_sort) : sig_sort :=
-  match sig_sort5 with
-  | (Cs A Rs) => Cs (open_tm_wrt_tm_rec k a5 A) Rs
-  | (Ax p a A R Rs) => Ax (open_tm_wrt_tm_rec k a5 p) (open_tm_wrt_tm_rec k a5 a) (open_tm_wrt_tm_rec k a5 A) R Rs
-end.
-
-Definition open_sort_wrt_tm_rec (k:nat) (a5:tm) (sort5:sort) : sort :=
-  match sort5 with
-  | (Tm A) => Tm (open_tm_wrt_tm_rec k a5 A)
-  | (Co phi) => Co (open_constraint_wrt_tm_rec k a5 phi)
 end.
 
 Definition open_sig_sort_wrt_co_rec (k:nat) (g5:co) (sig_sort5:sig_sort) : sig_sort :=
@@ -255,16 +245,10 @@ Definition open_sig_sort_wrt_co_rec (k:nat) (g5:co) (sig_sort5:sig_sort) : sig_s
   | (Ax p a A R Rs) => Ax (open_tm_wrt_co_rec k g5 p) (open_tm_wrt_co_rec k g5 a) (open_tm_wrt_co_rec k g5 A) R Rs
 end.
 
-Definition open_pattern_arg_wrt_co_rec (k:nat) (g5:co) (pattern_arg5:pattern_arg) : pattern_arg :=
-  match pattern_arg5 with
-  | (p_Tm nu a) => p_Tm nu (open_tm_wrt_co_rec k g5 a)
-  | (p_Co g) => p_Co (open_co_wrt_co_rec k g5 g)
-end.
-
-Definition open_sort_wrt_co_rec (k:nat) (g5:co) (sort5:sort) : sort :=
-  match sort5 with
-  | (Tm A) => Tm (open_tm_wrt_co_rec k g5 A)
-  | (Co phi) => Co (open_constraint_wrt_co_rec k g5 phi)
+Definition open_sig_sort_wrt_tm_rec (k:nat) (a5:tm) (sig_sort5:sig_sort) : sig_sort :=
+  match sig_sort5 with
+  | (Cs A Rs) => Cs (open_tm_wrt_tm_rec k a5 A) Rs
+  | (Ax p a A R Rs) => Ax (open_tm_wrt_tm_rec k a5 p) (open_tm_wrt_tm_rec k a5 a) (open_tm_wrt_tm_rec k a5 A) R Rs
 end.
 
 Definition open_pattern_arg_wrt_tm_rec (k:nat) (a5:tm) (pattern_arg5:pattern_arg) : pattern_arg :=
@@ -273,33 +257,51 @@ Definition open_pattern_arg_wrt_tm_rec (k:nat) (a5:tm) (pattern_arg5:pattern_arg
   | (p_Co g) => p_Co (open_co_wrt_tm_rec k a5 g)
 end.
 
-Definition open_co_wrt_tm a5 g_5 := open_co_wrt_tm_rec 0 g_5 a5.
+Definition open_sort_wrt_tm_rec (k:nat) (a5:tm) (sort5:sort) : sort :=
+  match sort5 with
+  | (Tm A) => Tm (open_tm_wrt_tm_rec k a5 A)
+  | (Co phi) => Co (open_constraint_wrt_tm_rec k a5 phi)
+end.
 
-Definition open_sig_sort_wrt_tm a5 sig_sort5 := open_sig_sort_wrt_tm_rec 0 sig_sort5 a5.
+Definition open_sort_wrt_co_rec (k:nat) (g5:co) (sort5:sort) : sort :=
+  match sort5 with
+  | (Tm A) => Tm (open_tm_wrt_co_rec k g5 A)
+  | (Co phi) => Co (open_constraint_wrt_co_rec k g5 phi)
+end.
 
-Definition open_sort_wrt_tm a5 sort5 := open_sort_wrt_tm_rec 0 sort5 a5.
+Definition open_pattern_arg_wrt_co_rec (k:nat) (g5:co) (pattern_arg5:pattern_arg) : pattern_arg :=
+  match pattern_arg5 with
+  | (p_Tm nu a) => p_Tm nu (open_tm_wrt_co_rec k g5 a)
+  | (p_Co g) => p_Co (open_co_wrt_co_rec k g5 g)
+end.
+
+Definition open_brs_wrt_tm a5 brs_6 := open_brs_wrt_tm_rec 0 brs_6 a5.
 
 Definition open_sig_sort_wrt_co g5 sig_sort5 := open_sig_sort_wrt_co_rec 0 sig_sort5 g5.
 
-Definition open_tm_wrt_co g5 a5 := open_tm_wrt_co_rec 0 a5 g5.
-
-Definition open_brs_wrt_co g5 brs_6 := open_brs_wrt_co_rec 0 brs_6 g5.
-
-Definition open_pattern_arg_wrt_co g5 pattern_arg5 := open_pattern_arg_wrt_co_rec 0 pattern_arg5 g5.
-
-Definition open_sort_wrt_co g5 sort5 := open_sort_wrt_co_rec 0 sort5 g5.
-
-Definition open_pattern_arg_wrt_tm a5 pattern_arg5 := open_pattern_arg_wrt_tm_rec 0 pattern_arg5 a5.
-
-Definition open_co_wrt_co g_5 g__6 := open_co_wrt_co_rec 0 g__6 g_5.
-
-Definition open_tm_wrt_tm a5 a_6 := open_tm_wrt_tm_rec 0 a_6 a5.
+Definition open_sig_sort_wrt_tm a5 sig_sort5 := open_sig_sort_wrt_tm_rec 0 sig_sort5 a5.
 
 Definition open_constraint_wrt_co g5 phi5 := open_constraint_wrt_co_rec 0 phi5 g5.
 
+Definition open_tm_wrt_co g5 a5 := open_tm_wrt_co_rec 0 a5 g5.
+
+Definition open_pattern_arg_wrt_tm a5 pattern_arg5 := open_pattern_arg_wrt_tm_rec 0 pattern_arg5 a5.
+
+Definition open_sort_wrt_tm a5 sort5 := open_sort_wrt_tm_rec 0 sort5 a5.
+
+Definition open_sort_wrt_co g5 sort5 := open_sort_wrt_co_rec 0 sort5 g5.
+
+Definition open_brs_wrt_co g5 brs_6 := open_brs_wrt_co_rec 0 brs_6 g5.
+
 Definition open_constraint_wrt_tm a5 phi5 := open_constraint_wrt_tm_rec 0 phi5 a5.
 
-Definition open_brs_wrt_tm a5 brs_6 := open_brs_wrt_tm_rec 0 brs_6 a5.
+Definition open_co_wrt_co g_5 g__6 := open_co_wrt_co_rec 0 g__6 g_5.
+
+Definition open_co_wrt_tm a5 g_5 := open_co_wrt_tm_rec 0 g_5 a5.
+
+Definition open_pattern_arg_wrt_co g5 pattern_arg5 := open_pattern_arg_wrt_co_rec 0 pattern_arg5 g5.
+
+Definition open_tm_wrt_tm a5 a_6 := open_tm_wrt_tm_rec 0 a_6 a5.
 
 (** terms are locally-closed pre-terms *)
 (** definitions *)
@@ -465,9 +467,8 @@ with lc_tm : tm -> Prop :=    (* defn lc_tm *)
  | lc_a_Sub : forall (R:role) (a:tm),
      (lc_tm a) ->
      (lc_tm (a_Sub R a))
- | lc_a_Coerce : forall (a:tm),
-     (lc_tm a) ->
-     (lc_tm (a_Coerce a))
+ | lc_a_Coerce : 
+     (lc_tm a_Coerce)
  | lc_a_SrcApp : forall (a b:tm),
      (lc_tm a) ->
      (lc_tm b) ->
@@ -562,7 +563,7 @@ with fv_tm_tm_tm (a5:tm) : vars :=
   | (a_DataCon K) => {}
   | (a_Case a brs5) => (fv_tm_tm_tm a) \u (fv_tm_tm_brs brs5)
   | (a_Sub R a) => (fv_tm_tm_tm a)
-  | (a_Coerce a) => (fv_tm_tm_tm a)
+  | a_Coerce => {}
   | (a_SrcApp a b) => (fv_tm_tm_tm a) \u (fv_tm_tm_tm b)
 end
 with fv_tm_tm_constraint (phi5:constraint) : vars :=
@@ -624,7 +625,7 @@ with fv_co_co_tm (a5:tm) : vars :=
   | (a_DataCon K) => {}
   | (a_Case a brs5) => (fv_co_co_tm a) \u (fv_co_co_brs brs5)
   | (a_Sub R a) => (fv_co_co_tm a)
-  | (a_Coerce a) => (fv_co_co_tm a)
+  | a_Coerce => {}
   | (a_SrcApp a b) => (fv_co_co_tm a) \u (fv_co_co_tm b)
 end
 with fv_co_co_constraint (phi5:constraint) : vars :=
@@ -723,7 +724,7 @@ with tm_subst_tm_tm (a5:tm) (x5:tmvar) (a_6:tm) {struct a_6} : tm :=
   | (a_DataCon K) => a_DataCon K
   | (a_Case a brs5) => a_Case (tm_subst_tm_tm a5 x5 a) (tm_subst_tm_brs a5 x5 brs5)
   | (a_Sub R a) => a_Sub R (tm_subst_tm_tm a5 x5 a)
-  | (a_Coerce a) => a_Coerce (tm_subst_tm_tm a5 x5 a)
+  | a_Coerce => a_Coerce 
   | (a_SrcApp a b) => a_SrcApp (tm_subst_tm_tm a5 x5 a) (tm_subst_tm_tm a5 x5 b)
 end
 with tm_subst_tm_constraint (a5:tm) (x5:tmvar) (phi5:constraint) {struct phi5} : constraint :=
@@ -785,7 +786,7 @@ with co_subst_co_tm (g5:co) (c5:covar) (a5:tm) {struct a5} : tm :=
   | (a_DataCon K) => a_DataCon K
   | (a_Case a brs5) => a_Case (co_subst_co_tm g5 c5 a) (co_subst_co_brs g5 c5 brs5)
   | (a_Sub R a) => a_Sub R (co_subst_co_tm g5 c5 a)
-  | (a_Coerce a) => a_Coerce (co_subst_co_tm g5 c5 a)
+  | a_Coerce => a_Coerce 
   | (a_SrcApp a b) => a_SrcApp (co_subst_co_tm g5 c5 a) (co_subst_co_tm g5 c5 b)
 end
 with co_subst_co_constraint (g5:co) (c5:covar) (phi5:constraint) {struct phi5} : constraint :=
@@ -956,38 +957,74 @@ Fixpoint A_snoc (xs : Apps) (x : App)  : Apps :=
   | A_cons y ys => (A_cons y (A_snoc ys x))
   end.
 
-
-(* -------------- A specific signature with Fix ------------ *)
-Definition Fix : atom.
-  pick fresh F.
-  exact F.
-Qed.
-
-Definition FixVar1 : atom.
- pick fresh F.
- exact F.
-Qed.
-
-Definition FixVar2 : atom.
- pick fresh F.
- exact F.
-Qed.
-
-Definition FixPat : tm := a_App (a_App (a_Fam Fix) (Rho Irrel) (a_Var_f FixVar1)) (Rho Rel) (a_Var_f FixVar2).
-
-Definition FixDef : tm := a_App (a_Var_f FixVar2) (Rho Rel) (a_App (a_App (a_Fam Fix) (Rho Irrel) a_Bullet) (Rho Rel) (a_Var_f FixVar2)).
-
-Definition FixTy : tm := a_Var_f FixVar1.
-
-Definition an_toplevel : sig := Fix ~ Ax FixPat FixDef FixTy Rep (Nom :: [Nom]).
-
-Definition toplevel : sig := erase_sig an_toplevel Nom.
-
 Fixpoint range (L : role_context) : roles :=
   match L with
   | nil => nil
   | (x,R) :: L' => range(L') ++ [ R ]
   end.
+
+
+(* -------------- A specific signature with Fix ------------ *)
+
+
+Definition constants :
+  { Star    : atom & 
+  { Fix     : atom &
+  { FixVar1 : atom &
+  { FixVar2 : atom &
+      Fix `notin` singleton Star /\
+      FixVar1 `notin` singleton Star  \u (singleton Fix) /\
+      FixVar2 `notin` singleton Star \u singleton Fix  \u singleton FixVar1  } } } }.
+Proof.
+  pick fresh Star.
+  pick fresh Fix.
+  pick fresh FixVar1.
+  pick fresh FixVar2.
+  exists Star.
+  exists Fix.
+  exists FixVar1.
+  exists FixVar2.
+  repeat split; auto.
+Defined.
+
+Definition Star : atom.
+  destruct constants as [s _].
+  exact s.
+Defined.
+
+Definition Fix : atom.
+  destruct constants as [_ [f _] ].
+  exact f.
+Defined.
+
+Lemma noteq : Star <> Fix.
+Proof.
+  unfold Star, Fix.
+  destruct constants as [s [f [f1 [f2 h] ] ] ].
+  destruct h as [g _].
+  fsetdec.
+Qed.
+
+Definition FixVar1 : atom.
+  destruct constants as [_ [_ [f1 _] ] ].
+  exact f1.
+Defined.
+
+Definition FixVar2 : atom.
+  destruct constants as [_ [_ [_ [f2 _] ] ] ].
+  exact f2.
+Defined.
+
+Definition FixPat : tm := a_App (a_App (a_Fam Fix) (Rho Irrel) a_Bullet) (Rho Rel) (a_Var_f FixVar2).
+
+Definition FixDef : tm := a_App (a_Var_f FixVar2) (Rho Rel)
+                              (a_App (a_App (a_Fam Fix) (Rho Irrel) a_Bullet) (Rho Rel) (a_Var_f FixVar2)).
+
+Definition FixTy : tm  := a_Pi Irrel a_Star 
+                             (a_Pi Rel (a_Pi Rel (a_Var_b 0) (a_Var_b 1)) (a_Var_b 1)).
+
+Definition toplevel : sig := Fix ~ Ax FixPat FixDef FixTy Rep (Nom :: [Nom]).
+
 
 
 
@@ -1014,10 +1051,14 @@ Inductive RolePath : tm -> const -> roles -> Prop :=    (* defn RolePath *)
  | RolePath_Const : forall (F:const) (Rs:roles) (p a A:tm) (R1:role),
       binds  F  ( (Ax p a A R1 Rs) )   toplevel   ->
      RolePath (a_Fam F) F Rs
- | RolePath_App : forall (a:tm) (R1:role) (b':tm) (F:const) (Rs:roles),
+ | RolePath_TApp : forall (a:tm) (R1:role) (b':tm) (F:const) (Rs:roles),
      lc_tm b' ->
      RolePath a F  ( R1 :: Rs )  ->
      RolePath  ( (a_App a (Role R1) b') )  F Rs
+ | RolePath_App : forall (a b':tm) (F:const) (Rs:roles),
+     lc_tm b' ->
+     RolePath a F Rs ->
+     RolePath  ( (a_App a (Rho Rel) b') )  F Rs
  | RolePath_IApp : forall (a:tm) (F:const) (Rs:roles),
      RolePath a F Rs ->
      RolePath  ( (a_App a (Rho Irrel) a_Bullet) )  F Rs
@@ -1050,9 +1091,12 @@ Inductive AppsPath : role -> tm -> const -> Apps -> Prop :=    (* defn AppsPath 
 Inductive AppRoles : Apps -> roles -> Prop :=    (* defn AppRoles *)
  | AR_nil : 
      AppRoles A_nil  nil 
- | AR_consApp : forall (R1:role) (Apps5:Apps) (Rs:roles),
+ | AR_consTApp : forall (R1:role) (Apps5:Apps) (Rs:roles),
      AppRoles Apps5 Rs ->
      AppRoles (A_cons (A_Tm (Role R1)) Apps5)  ( R1 :: Rs ) 
+ | AR_consApp : forall (Apps5:Apps) (Rs:roles),
+     AppRoles Apps5 Rs ->
+     AppRoles (A_cons (A_Tm (Rho Rel)) Apps5) Rs
  | AR_consIApp : forall (Apps5:Apps) (Rs:roles),
      AppRoles Apps5 Rs ->
      AppRoles (A_cons (A_Tm (Rho Irrel)) Apps5) Rs
@@ -1071,19 +1115,19 @@ with SatApp : const -> Apps -> Prop :=    (* defn SatApp *)
      SatApp F Apps5.
 
 (* defns JPatCtx *)
-Inductive PatternContexts : role_context -> context -> const -> tm -> tm -> tm -> Prop :=    (* defn PatternContexts *)
+Inductive PatternContexts : role_context -> context -> available_props -> const -> tm -> tm -> tm -> Prop :=    (* defn PatternContexts *)
  | PatCtx_Const : forall (F:const) (A:tm),
      lc_tm A ->
-     PatternContexts  nil   nil  F A (a_Fam F) A
- | PatCtx_PiRel : forall (L:vars) (W:role_context) (R:role) (G:context) (A':tm) (F:const) (B p A:tm),
-     PatternContexts W G F B p (a_Pi Rel A' A) ->
-      ( forall x , x \notin  L  -> PatternContexts  (( x  ~  R ) ++  W )   (( x ~ Tm  A' ) ++  G )  F B (a_App p (Role R) (a_Var_f x))  ( open_tm_wrt_tm A (a_Var_f x) )  ) 
- | PatCtx_PiIrr : forall (L:vars) (W:role_context) (G:context) (A':tm) (F:const) (B p A:tm),
-     PatternContexts W G F B p (a_Pi Irrel A' A) ->
-      ( forall x , x \notin  L  -> PatternContexts W  (( x ~ Tm  A' ) ++  G )  F B (a_App p (Rho Irrel) a_Bullet)  ( open_tm_wrt_tm A (a_Var_f x) )  ) 
- | PatCtx_CPi : forall (L:vars) (W:role_context) (G:context) (phi:constraint) (F:const) (B p A:tm),
-     PatternContexts W G F B p (a_CPi phi A) ->
-      ( forall c , c \notin  L  -> PatternContexts W  (( c ~ Co  phi ) ++  G )  F B (a_CApp p g_Triv)  ( open_tm_wrt_co A (g_Var_f c) )  ) .
+     PatternContexts  nil   nil   AtomSetImpl.empty  F A (a_Fam F) A
+ | PatCtx_PiRel : forall (L:vars) (W:role_context) (R:role) (G:context) (A':tm) (D:available_props) (F:const) (B p A:tm),
+     PatternContexts W G D F B p (a_Pi Rel A' A) ->
+      ( forall x , x \notin  L  -> PatternContexts  (( x  ~  R ) ++  W )   (( x ~ Tm  A' ) ++  G )  D F B (a_App p (Role R) (a_Var_f x))  ( open_tm_wrt_tm A (a_Var_f x) )  ) 
+ | PatCtx_PiIrr : forall (L:vars) (W:role_context) (G:context) (A':tm) (D:available_props) (F:const) (B p A:tm),
+     PatternContexts W G D F B p (a_Pi Irrel A' A) ->
+      ( forall x , x \notin  L  -> PatternContexts W  (( x ~ Tm  A' ) ++  G )   (singleton  x  \u  D )  F B (a_App p (Rho Irrel) a_Bullet)  ( open_tm_wrt_tm A (a_Var_f x) )  ) 
+ | PatCtx_CPi : forall (L:vars) (W:role_context) (G:context) (phi:constraint) (D:available_props) (F:const) (B p A:tm),
+     PatternContexts W G D F B p (a_CPi phi A) ->
+      ( forall c , c \notin  L  -> PatternContexts W  (( c ~ Co  phi ) ++  G )  D F B (a_CApp p g_Triv)  ( open_tm_wrt_co A (g_Var_f c) )  ) .
 
 (* defns JRename *)
 Inductive Rename : tm -> tm -> tm -> tm -> available_props -> available_props -> Prop :=    (* defn Rename *)
@@ -1117,15 +1161,6 @@ Inductive MatchSubst : tm -> tm -> tm -> tm -> Prop :=    (* defn MatchSubst *)
  | MatchSubst_CApp : forall (a1 a2 b1 b2:tm),
      MatchSubst a1 a2 b1 b2 ->
      MatchSubst  ( (a_CApp a1 g_Triv) )   ( (a_CApp a2 g_Triv) )  b1 b2.
-
-(* defns JPatData *)
-Inductive PatData : tm -> const -> pattern_args -> Prop :=    (* defn PatData *)
- | PatData_Head : forall (F:const),
-     PatData (a_Fam F) F  nil 
- | PatData_Rel : forall (p:tm) (R:role) (a:tm) (F:const) (PA:pattern_args),
-     lc_tm a ->
-     PatData p F PA ->
-     PatData  ( (a_App p (Role R) a) )  F  (cons  (p_Tm (Role R) a)   PA ) .
 
 (* defns JIsPattern *)
 Inductive Pattern : tm -> Prop :=    (* defn Pattern *)
@@ -1542,25 +1577,24 @@ with reduction : tm -> tm -> role -> Prop :=    (* defn reduction *)
 
 (* defns JBranchTyping *)
 Inductive BranchTyping : context -> Apps -> role -> tm -> tm -> tm -> pattern_args -> tm -> tm -> tm -> Prop :=    (* defn BranchTyping *)
- | BranchTyping_Base : forall (L:vars) (G:context) (a A b:tm) (pattern_args5:pattern_args) (C:tm),
-     lc_tm C  ->
+ | BranchTyping_Base : forall (G:context) (a A b:tm) (pattern_args5:pattern_args) (C1 C2:tm),
      lc_tm a ->
      lc_tm b ->
      lc_tm A ->
-     lc_tm (a_CPi  ( (Eq a  (apply_pattern_args  b   pattern_args5 )  A Nom) )  C) ->
       uniq  G  ->
-      ( forall c , c \notin  L  -> BranchTyping G A_nil Nom a A b pattern_args5 A (a_CPi  ( (Eq a  (apply_pattern_args  b   pattern_args5 )  A Nom) )  C)  ( open_tm_wrt_co C (g_Var_f c) )  ) 
+      (  (open_tm_wrt_co  C1   g_Triv )   =  C2 )  ->
+     BranchTyping G A_nil Nom a A b pattern_args5 A (a_CPi  ( (Eq a  (apply_pattern_args  b   pattern_args5 )  A Nom) )  C1) C2
  | BranchTyping_PiRole : forall (L:vars) (G:context) (R:role) (Apps5:Apps) (a A1 b:tm) (pattern_args5:pattern_args) (A B C C':tm),
-      ( forall x , x \notin  L  -> BranchTyping  (( x ~ Tm  A ) ++  G )  Apps5 Nom a A1 b  (cons  (p_Tm (Role R) (a_Var_f x))   pattern_args5 )   ( open_tm_wrt_tm B (a_Var_f x) )   ( open_tm_wrt_tm C (a_Var_f x) )  C' )  ->
+      ( forall x , x \notin  L  -> BranchTyping  (( x ~ Tm  A ) ++  G )  Apps5 Nom a A1 b  ( pattern_args5  ++ [  (p_Tm (Role R) (a_Var_f x))  ])   ( open_tm_wrt_tm B (a_Var_f x) )   ( open_tm_wrt_tm C (a_Var_f x) )  C' )  ->
      BranchTyping G  ( (A_cons (A_Tm (Role R)) Apps5) )  Nom a A1 b pattern_args5 (a_Pi Rel A B) (a_Pi Rel A C) C'
  | BranchTyping_PiRel : forall (L:vars) (G:context) (Apps5:Apps) (a A1 b:tm) (pattern_args5:pattern_args) (A B C C':tm),
-      ( forall x , x \notin  L  -> BranchTyping  (( x ~ Tm  A ) ++  G )  Apps5 Nom a A1 b  (cons  (p_Tm (Rho Rel) (a_Var_f x))   pattern_args5 )   ( open_tm_wrt_tm B (a_Var_f x) )   ( open_tm_wrt_tm C (a_Var_f x) )  C' )  ->
+      ( forall x , x \notin  L  -> BranchTyping  (( x ~ Tm  A ) ++  G )  Apps5 Nom a A1 b  ( pattern_args5  ++ [  (p_Tm (Rho Rel) (a_Var_f x))  ])   ( open_tm_wrt_tm B (a_Var_f x) )   ( open_tm_wrt_tm C (a_Var_f x) )  C' )  ->
      BranchTyping G  ( (A_cons (A_Tm (Rho Rel)) Apps5) )  Nom a A1 b pattern_args5 (a_Pi Rel A B) (a_Pi Rel A C) C'
  | BranchTyping_PiIrrel : forall (L:vars) (G:context) (Apps5:Apps) (a A1 b:tm) (pattern_args5:pattern_args) (A B C C':tm),
-      ( forall x , x \notin  L  -> BranchTyping  (( x ~ Tm  A ) ++  G )  Apps5 Nom a A1 b  (cons  (p_Tm (Rho Irrel) a_Bullet)   pattern_args5 )   ( open_tm_wrt_tm B (a_Var_f x) )   ( open_tm_wrt_tm C (a_Var_f x) )  C' )  ->
+      ( forall x , x \notin  L  -> BranchTyping  (( x ~ Tm  A ) ++  G )  Apps5 Nom a A1 b  ( pattern_args5  ++ [  (p_Tm (Rho Irrel) a_Bullet)  ])   ( open_tm_wrt_tm B (a_Var_f x) )   ( open_tm_wrt_tm C (a_Var_f x) )  C' )  ->
      BranchTyping G  ( (A_cons (A_Tm (Rho Irrel)) Apps5) )  Nom a A1 b pattern_args5 (a_Pi Irrel A B) (a_Pi Irrel A C) C'
  | BranchTyping_CPi : forall (L:vars) (G:context) (Apps5:Apps) (a A b:tm) (pattern_args5:pattern_args) (phi:constraint) (B C C':tm),
-      ( forall c , c \notin  L  -> BranchTyping  (( c ~ Co  phi ) ++  G )  Apps5 Nom a A b  (cons  (p_Co g_Triv)   pattern_args5 )   ( open_tm_wrt_co B (g_Var_f c) )   ( open_tm_wrt_co C (g_Var_f c) )  C' )  ->
+      ( forall c , c \notin  L  -> BranchTyping  (( c ~ Co  phi ) ++  G )  Apps5 Nom a A b  ( pattern_args5  ++ [  (p_Co g_Triv)  ])   ( open_tm_wrt_co B (g_Var_f c) )   ( open_tm_wrt_co C (g_Var_f c) )  C' )  ->
      BranchTyping G  ( (A_cons A_Co Apps5) )  Nom a A b pattern_args5 (a_CPi phi B) (a_CPi phi C) C'.
 
 (* defns Jett *)
@@ -1690,11 +1724,11 @@ with DefEq : context -> available_props -> tm -> tm -> tm -> role -> Prop :=    
      DefEq G D a1 b1  ( (a_Pi Rel A B) )  R' ->
      DefEq G D a2 b2 A Nom ->
      DefEq G D (a_App a1 (Rho Rel) a2) (a_App b1 (Rho Rel) b2)  (  (open_tm_wrt_tm  B   a2 )  )  R'
- | E_TAppCong : forall (G:context) (D:available_props) (a1:tm) (R:role) (a2 b1 b2 B:tm) (R':role) (A:tm) (F:const) (Rs:roles) (F':const) (Rs':roles),
+ | E_TAppCong : forall (G:context) (D:available_props) (a1:tm) (R:role) (a2 b1 b2 B:tm) (R':role) (A:tm) (F:const) (Rs:roles),
      DefEq G D a1 b1  ( (a_Pi Rel A B) )  R' ->
      DefEq G D a2 b2 A  (param R   R' )  ->
      RolePath a1 F  ( R :: Rs )  ->
-     RolePath b1 F'  ( R :: Rs' )  ->
+     RolePath b1 F  ( R :: Rs )  ->
      Typing G (a_App b1 (Role R) b2)  (open_tm_wrt_tm  B   a2 )  ->
      DefEq G D (a_App a1 (Role R) a2) (a_App b1 (Role R) b2)  (  (open_tm_wrt_tm  B   a2 )  )  R'
  | E_IAppCong : forall (G:context) (D:available_props) (a1 b1 B a:tm) (R':role) (A:tm),
@@ -1721,12 +1755,12 @@ with DefEq : context -> available_props -> tm -> tm -> tm -> role -> Prop :=    
      DefEq G D  ( (a_UCAbs a) )   ( (a_UCAbs b) )  (a_CPi phi1 B) R
  | E_CAppCong : forall (G:context) (D:available_props) (a1 b1 B:tm) (R':role) (a b A:tm) (R:role),
      DefEq G D a1 b1  ( (a_CPi  ( (Eq a b A R) )  B) )  R' ->
-     DefEq G  (dom  G )  a b A  (param R   R' )  ->
+     DefEq G  (dom  G )  a b A R ->
      DefEq G D (a_CApp a1 g_Triv) (a_CApp b1 g_Triv)  (  (open_tm_wrt_co  B   g_Triv )  )  R'
  | E_CPiSnd : forall (G:context) (D:available_props) (B1 B2:tm) (R0:role) (a1 a2 A:tm) (R:role) (a1' a2' A':tm) (R':role),
      DefEq G D (a_CPi  ( (Eq a1 a2 A R) )  B1) (a_CPi  ( (Eq a1' a2' A' R') )  B2) a_Star R0 ->
-     DefEq G  (dom  G )  a1 a2 A  (param R   R0 )  ->
-     DefEq G  (dom  G )  a1' a2' A'  (param R'   R0 )  ->
+     DefEq G  (dom  G )  a1 a2 A R ->
+     DefEq G  (dom  G )  a1' a2' A' R' ->
      DefEq G D  (open_tm_wrt_co  B1   g_Triv )   (open_tm_wrt_co  B2   g_Triv )  a_Star R0
  | E_Cast : forall (G:context) (D:available_props) (a' b' A':tm) (R':role) (a b A:tm) (R:role),
      DefEq G D a b A R ->
@@ -1740,18 +1774,19 @@ with DefEq : context -> available_props -> tm -> tm -> tm -> role -> Prop :=    
  | E_IsoSnd : forall (G:context) (D:available_props) (A A' a b:tm) (R1:role) (a' b':tm),
      Iso G D (Eq a b A R1) (Eq a' b' A' R1) ->
      DefEq G D A A' a_Star Rep
- | E_PatCong : forall (G:context) (D:available_props) (a:tm) (F:const) (Apps5:Apps) (b1 b2 a' b1' b2' C:tm) (R0:role) (A B A1:tm),
+ | E_PatCong : forall (G:context) (D:available_props) (a:tm) (F:const) (Apps5:Apps) (b1 b2 a' b1' b2' C:tm) (R0:role) (A B A1 B':tm),
      DefEq G D a a' A Nom ->
      DefEq G D b1 b1' B R0 ->
      DefEq G D b2 b2' C R0 ->
      BranchTyping G Apps5 Nom a A (a_Fam F)  nil  A1 B C ->
-     BranchTyping G Apps5 Nom a' A (a_Fam F)  nil  A1 B C ->
+     BranchTyping G Apps5 Nom a' A (a_Fam F)  nil  A1 B' C ->
+     DefEq G D B B' a_Star Rep ->
      SatApp F Apps5 ->
      Typing G (a_Fam F) A1 ->
      DefEq G D (a_Pattern Nom a F Apps5 b1 b2) (a_Pattern Nom a' F Apps5 b1' b2') C R0
- | E_LeftRel : forall (G:context) (D:available_props) (a a' A B:tm) (R':role) (F:const) (b b':tm) (R1:role),
-     ValuePath a F ->
-     ValuePath a' F ->
+ | E_LeftRel : forall (G:context) (D:available_props) (a a' A B:tm) (R' R1:role) (b:tm) (F:const) (b':tm),
+     CasePath R'  ( (a_App a (Role R1) b) )  F ->
+     CasePath R'  ( (a_App a' (Role R1) b') )  F ->
      Typing G a (a_Pi Rel A B) ->
      Typing G b A ->
      Typing G a' (a_Pi Rel A B) ->
@@ -1760,8 +1795,8 @@ with DefEq : context -> available_props -> tm -> tm -> tm -> role -> Prop :=    
      DefEq G  (dom  G )   (open_tm_wrt_tm  B   b )   (open_tm_wrt_tm  B   b' )  a_Star Rep ->
      DefEq G D a a' (a_Pi Rel A B) R'
  | E_LeftIrrel : forall (G:context) (D:available_props) (a a' A B:tm) (R':role) (F:const) (b b':tm),
-     ValuePath a F ->
-     ValuePath a' F ->
+     CasePath R'  ( (a_App a (Rho Irrel) a_Bullet) )  F ->
+     CasePath R'  ( (a_App a' (Rho Irrel) a_Bullet) )  F ->
      Typing G a (a_Pi Irrel A B) ->
      Typing G b A ->
      Typing G a' (a_Pi Irrel A B) ->
@@ -1770,8 +1805,8 @@ with DefEq : context -> available_props -> tm -> tm -> tm -> role -> Prop :=    
      DefEq G  (dom  G )   (open_tm_wrt_tm  B   b )   (open_tm_wrt_tm  B   b' )  a_Star Rep ->
      DefEq G D a a' (a_Pi Irrel A B) R'
  | E_Right : forall (G:context) (D:available_props) (b b' A:tm) (R1 R':role) (a:tm) (F:const) (a' B:tm),
-     ValuePath a F ->
-     ValuePath a' F ->
+     CasePath R'  ( (a_App a (Role R1) b) )  F ->
+     CasePath R'  ( (a_App a' (Role R1) b') )  F ->
      Typing G a (a_Pi Rel A B) ->
      Typing G b A ->
      Typing G a' (a_Pi Rel A B) ->
@@ -1780,8 +1815,8 @@ with DefEq : context -> available_props -> tm -> tm -> tm -> role -> Prop :=    
      DefEq G  (dom  G )   (open_tm_wrt_tm  B   b )   (open_tm_wrt_tm  B   b' )  a_Star Rep ->
      DefEq G D b b' A  (param R1   R' ) 
  | E_CLeft : forall (G:context) (D:available_props) (a a' a1 a2 A:tm) (R1:role) (B:tm) (R':role) (F:const),
-     ValuePath a F ->
-     ValuePath a' F ->
+     CasePath R'  ( (a_CApp a g_Triv) )  F ->
+     CasePath R'  ( (a_CApp a' g_Triv) )  F ->
      Typing G a (a_CPi  ( (Eq a1 a2 A R1) )  B) ->
      Typing G a' (a_CPi  ( (Eq a1 a2 A R1) )  B) ->
      DefEq G  (dom  G )  a1 a2 A  (param R1   R' )  ->
@@ -1810,12 +1845,13 @@ Inductive Sig : sig -> Prop :=    (* defn Sig *)
      Typing  nil  A a_Star ->
       ~ AtomSetImpl.In  F  (dom  S )  ->
      Sig  (( F ~ (Cs A Rs) )++ S ) 
- | Sig_ConsAx : forall (S:sig) (F:const) (p a A:tm) (R:role) (W:role_context) (G:context) (B:tm),
+ | Sig_ConsAx : forall (S:sig) (F:const) (p a A:tm) (R:role) (W:role_context) (G:context) (D:available_props) (B:tm),
      Sig S ->
       ~ AtomSetImpl.In  F  (dom  S )  ->
      Typing  nil  A a_Star ->
-     PatternContexts W G F A p B ->
+     PatternContexts W G D F A p B ->
      Typing G a B ->
+      (AtomSetImpl.For_all (fun x => x `notin`   (fv_tm_tm_tm  a )  )  D  )  ->
      roleing W a R ->
      Sig  (( F ~ (Ax p a A R  (range( W )) ) )++ S ) .
 
@@ -1886,7 +1922,7 @@ Inductive SrcTyping : context -> tm -> tm -> Prop :=    (* defn SrcTyping *)
  | S_Coerce : forall (G:context) (a B A:tm),
      SrcTyping G a A ->
      DefEq G  (dom  G )  A B a_Star Rep ->
-     SrcTyping G (a_Coerce a) B
+     SrcTyping G (a_SrcApp a_Coerce a) B
  | S_App : forall (G:context) (b a B a' A:tm),
      SrcTyping G b (a_Pi Rel A B) ->
      SrcTrans G a a' A ->
@@ -1961,7 +1997,7 @@ with SrcTrans : context -> tm -> tm -> tm -> Prop :=    (* defn SrcTrans *)
  | ST_Coerce : forall (G:context) (a a' B A:tm),
      SrcTrans G a a' A ->
      DefEq G  (dom  G )  A B a_Star Rep ->
-     SrcTrans G (a_Coerce a) a' B
+     SrcTrans G (a_SrcApp a_Coerce a) a' B
  | ST_CPi : forall (L:vars) (G:context) (phi:constraint) (B B':tm) (phi':constraint),
      SrcPropWff G phi phi' ->
       ( forall c , c \notin  L  -> SrcTrans  (( c ~ Co  phi' ) ++  G )   ( open_tm_wrt_co B (g_Var_f c) )   ( open_tm_wrt_co B' (g_Var_f c) )  a_Star )  ->
@@ -2004,6 +2040,6 @@ Inductive head_reduction : context -> tm -> tm -> role -> Prop :=    (* defn hea
 
 
 (** infrastructure *)
-Hint Constructors SubRole RolePath AppsPath AppRoles SatApp PatternContexts Rename MatchSubst PatData Pattern SubPat tm_pattern_agree tm_subpattern_agree subtm_pattern_agree ValuePath CasePath ApplyArgs Value value_type consistent roleing RhoCheck Par MultiPar joins Beta reduction_in_one reduction BranchTyping PropWff Typing Iso DefEq Ctx Sig RoleWeaken SigWeaken SrcTyping SrcTrans SrcPropWff AnnPropWff AnnTyping AnnIso AnnDefEq AnnCtx head_reduction lc_co lc_brs lc_tm lc_constraint lc_sort lc_pattern_arg lc_sig_sort.
+Hint Constructors SubRole RolePath AppsPath AppRoles SatApp PatternContexts Rename MatchSubst Pattern SubPat tm_pattern_agree tm_subpattern_agree subtm_pattern_agree ValuePath CasePath ApplyArgs Value value_type consistent roleing RhoCheck Par MultiPar joins Beta reduction_in_one reduction BranchTyping PropWff Typing Iso DefEq Ctx Sig RoleWeaken SigWeaken SrcTyping SrcTrans SrcPropWff AnnPropWff AnnTyping AnnIso AnnDefEq AnnCtx head_reduction lc_co lc_brs lc_tm lc_constraint lc_sort lc_pattern_arg lc_sig_sort.
 
 
